Mid spec

src/specs/AddAssignPermutationLinearisationContributionWithV.ec
@@ -7,6 +7,8 @@ require import Verifier.
 require import VerifierConsts.
 require import YulPrimops.
 
+import MemoryMap.
+
 module AddAssignPermutationLinearisationContributionWithV = {
   proc low(dest : uint256, stateOpening0AtZ : uint256, stateOpening1AtZ : uint256, stateOpening2AtZ : uint256, stateOpening3AtZ : uint256): unit = {
     var factor, _1, _3, gamma, _4, intermediateValue, _6, _7, _9, _10, _12, _13, l0AtZ, _16, _17, _18, _20, _21, _23, beta', gamma_1, _25, _26, _27, intermediateValue_1, _29, _30, _31, _33, _34, _35, _36;
@@ -64,47 +66,42 @@ module AddAssignPermutationLinearisationContributionWithV = {
     PointSubAssign.low(dest, QUERIES_BUFFER_POINT_SLOT);
   }
 
-  proc mid(dest : uint256, stateOpening0AtZ : uint256, stateOpening1AtZ : uint256, stateOpening2AtZ : uint256, stateOpening3AtZ : uint256, factor: int, state_beta: int, state_z: int, state_gamma: int): unit = {
-    var factor, _1, _3, gamma, _4, intermediateValue, _6, _7, _9, _10, _12, _13, l0AtZ, _16, _17, _18, _20, _21, _23, beta', gamma_1, _25, _26, _27, intermediateValue_1, _29, _30, _31, _33, _34, _35, _36;
-    factor <- ((
-      factor *
-      (state_z * state_beta + state_gamma + stateOpening0AtZ) *
-      (state_z * state_beta * Constants.NON_RESIDUE_0 + state_gamma + stateOpening1AtZ) *
-      (state_z * state_beta * Constants.NON_RESIDUE_1 + state_gamma + stateOpening2AtZ) *
-      (state_z * state_beta * Constants.NON_RESIDUE_2 + state_gamma + stateOpening3AtZ) +
-      state_l0AtZ * state_alpha5
+  proc mid(point: (int*int), vk_permutation_3: (int*int), stateOpening0AtZ: int, stateOpening1AtZ: int, stateOpening2AtZ: int, stateOpening3AtZ: int, state_beta: int, state_v: int, state_z: int, state_gamma: int, state_alpha4: int, state_alpha5: int, state_gp_omega: int, state_l0AtZ: int, poly0_opening: int, poly1_opening: int, poly2_opening: int): (int * (int*int)) option = {
+      var mul_factor, buffer_point, ret_point, ret_factor,
+      ret;
+    mul_factor <- ((
+      (state_alpha4 * state_beta * state_gp_omega) *
+      ((poly0_opening * state_beta) + state_gamma + stateOpening0AtZ) *
+      ((poly1_opening * state_beta) + state_gamma + stateOpening1AtZ) *
+      ((poly2_opening * state_beta) + state_gamma + stateOpening2AtZ)
     ) * state_v) %% Constants.R;
-    Primops.mstore(COPY_PERMUTATION_FIRST_AGGREGATED_COMMITMENT_COEFF, factor);
-    _20 <@ Primops.mload(STATE_BETA_SLOT);
-    _21 <@ Primops.mload(STATE_POWER_OF_ALPHA_4_SLOT);
-    factor <- (PurePrimops.mulmod _21 _20 Constants.R);
-    _23 <@ Primops.mload(PROOF_COPY_PERMUTATION_GRAND_PRODUCT_OPENING_AT_Z_OMEGA_SLOT);
-    factor <- (PurePrimops.mulmod factor _23 Constants.R);
-    beta' <@ Primops.mload(STATE_BETA_SLOT);
-    gamma_1 <@ Primops.mload(STATE_GAMMA_SLOT);
-    _25 <@ Primops.mload(PROOF_COPY_PERMUTATION_POLYS_0_OPENING_AT_Z_SLOT);
-    _26 <- (PurePrimops.mulmod _25 beta' Constants.R);
-    _27 <- (PurePrimops.addmod _26 gamma_1 Constants.R);
-    intermediateValue_1 <- (PurePrimops.addmod _27 stateOpening0AtZ Constants.R);
-    factor <- (PurePrimops.mulmod factor intermediateValue_1 Constants.R);
-    _29 <@ Primops.mload(PROOF_COPY_PERMUTATION_POLYS_1_OPENING_AT_Z_SLOT);
-    _30 <- (PurePrimops.mulmod _29 beta' Constants.R);
-    _31 <- (PurePrimops.addmod _30 gamma_1 Constants.R);
-    intermediateValue_1 <- (PurePrimops.addmod _31 stateOpening1AtZ Constants.R);
-    factor <- (PurePrimops.mulmod factor intermediateValue_1 Constants.R);
-    _33 <@ Primops.mload(PROOF_COPY_PERMUTATION_POLYS_2_OPENING_AT_Z_SLOT);
-    _34 <- (PurePrimops.mulmod _33 beta' Constants.R);
-    _35 <- (PurePrimops.addmod _34 gamma_1 Constants.R);
-    intermediateValue_1 <- (PurePrimops.addmod _35 stateOpening2AtZ Constants.R);
-    factor <- (PurePrimops.mulmod factor intermediateValue_1 Constants.R);
-    _36 <@ Primops.mload(STATE_V_SLOT);
-    factor <- (PurePrimops.mulmod factor _36 Constants.R);
-    PointMulIntoDest.low(VK_PERMUTATION_3_X_SLOT, factor, QUERIES_BUFFER_POINT_SLOT);
-    PointSubAssign.low(dest, QUERIES_BUFFER_POINT_SLOT);
+    buffer_point <@ PointMulIntoDest.mid(vk_permutation_3.`1, vk_permutation_3.`2, mul_factor);
+    if (is_none buffer_point) {
+      ret_point <- None;
+    } else {
+      ret_point <@ PointSubAssign.mid(point, odflt (0,0) buffer_point);
+    }
+
+    if (is_none ret_point) {
+      ret <- None;
+    } else {
+      ret_factor <- ((
+        state_alpha4 *
+        (state_z * state_beta + state_gamma + stateOpening0AtZ) *
+        (state_z * state_beta * Constants.NON_RESIDUE_0 + state_gamma + stateOpening1AtZ) *
+        (state_z * state_beta * Constants.NON_RESIDUE_1 + state_gamma + stateOpening2AtZ) *
+        (state_z * state_beta * Constants.NON_RESIDUE_2 + state_gamma + stateOpening3AtZ) +
+        state_l0AtZ * state_alpha5
+      ) * state_v) %% Constants.R;
+      ret <- Some (ret_factor, odflt (0, 0) ret_point);
+    }
+
+    return ret;
   }
 }.
 
-lemma addAssignPermutationLinearisationContributionWithV_extracted_equiv_low :
+(* requries sub assign extracted fix *)
+(* lemma addAssignPermutationLinearisationContributionWithV_extracted_equiv_low :
     equiv [
       Verifier_1261.usr_addAssignPermutationLinearisationContributionWithV ~ AddAssignPermutationLinearisationContributionWithV.low :
       ={arg, glob AddAssignPermutationLinearisationContributionWithV} ==>
@@ -115,4 +112,35 @@ proof.
   call (pointSubAssign_extracted_equiv_low). wp.
   call (pointMulIntoDest_extracted_equiv_low).
   inline*. wp. skip. rewrite /Constants.R. by progress.
-qed.
+qed. *)
+
+lemma addAssignPermutationLinearisationContributionWithV_low_equiv_mid (mem_0: mem) :
+    equiv [
+      AddAssignPermutationLinearisationContributionWithV.low ~ AddAssignPermutationLinearisationContributionWithV.mid :
+      arg{2}.`1.`1 = W256.to_uint (load mem_0 arg{1}.`1) /\
+      arg{2}.`1.`2 = W256.to_uint (load mem_0 (arg{1}.`1 + W256.of_int 32)) /\
+      arg{2}.`2.`1 = W256.to_uint (load mem_0 VK_PERMUTATION_3_X_SLOT) /\
+      arg{2}.`2.`2 = W256.to_uint (load mem_0 VK_PERMUTATION_3_Y_SLOT) /\
+      arg{2}.`3 = W256.to_uint arg{1}.`2 /\
+      arg{2}.`4 = W256.to_uint arg{1}.`3 /\
+      arg{2}.`5 = W256.to_uint arg{1}.`4 /\
+      arg{2}.`6 = W256.to_uint arg{1}.`5 /\
+      arg{2}.`7 = W256.to_uint (load mem_0 STATE_BETA_SLOT)
+    ].
+
+
+
+
+
+
+
+
+
+
+
+
+
+
+
+
+
